Saving some work

src/ManCompSoundness.v
@@ -2,39 +2,116 @@
       Namely, that the compiler outputs a collection of manifests that support 
       execution of the input protocols.  *)
 
-Require Import Manifest Manifest_Compiler Manifest_Generator ID_Type
+Require Import Manifest Manifest_Generator ID_Type
   Maps Term_Defs List Cvm_St Cvm_Impl ErrorStMonad_Coq StructTactics 
   Cvm_Monad EqClass Manifest_Admits Auto.
-Require Import Manifest_Generator_Facts Eqb_Evidence.
+Require Import Manifest_Generator_Facts Eqb_Evidence Attestation_Session.
 
-Require Import Manifest_Generator_Helpers ManCompSoundness_Helpers.
+Require Import Manifest_Generator_Helpers Session_Config_Compiler.
+Require Import Helpers_CvmSemantics.
 
 Require Import Coq.Program.Tactics.
 
 Import ListNotations.
 
-(* Set Nested Proofs Allowed. *)
+Definition session_config_subset (sc1 sc2 : Session_Config) : Prop :=
+  (forall aid l targ targid ev, 
+      (forall res, 
+      sc1.(aspCb) (asp_paramsC aid l targ targid) ev = resultC res ->
+      sc2.(aspCb) (asp_paramsC aid l targ targid) ev = resultC res)) /\
+  (forall p, (forall res, 
+      map_get (sc1.(plc_map)) p = Some res ->
+      map_get (sc2.(plc_map)) p = Some res)) /\
+  (forall p, (forall res, 
+      map_get (sc1.(pubkey_map)) p = Some res ->
+      map_get (sc2.(pubkey_map)) p = Some res)) /\
+  (forall aid l targ targid ev errStr,
+      sc1.(aspCb) (asp_paramsC aid l targ targid) ev = errC (Runtime errStr) ->
+      sc2.(aspCb) (asp_paramsC aid l targ targid) ev = errC (Runtime errStr)) 
+  /\
+  (forall p,
+      map_get (sc1.(plc_map)) p = None ->
+      map_get (sc2.(plc_map)) p = None) /\
+  (forall p, 
+      map_get (sc1.(pubkey_map)) p = None ->
+      map_get (sc2.(pubkey_map)) p = None).
 
+Theorem session_config_subset_refl : forall sc1,
+  session_config_subset sc1 sc1.
+Proof.
+  unfold session_config_subset; intuition.
+Qed.
 
-Definition lib_supports_manifest (al : AM_Library) (am : Manifest) : Prop :=
-  (forall (a : ASP_ID), In_set a am.(asps) -> 
-    exists aloc, Maps.map_get al.(Lib_ASPs) a = Some aloc) /\
-  (forall (up : Plc), In_set up am.(uuidPlcs) -> 
-    exists b, Maps.map_get al.(Lib_Plcs) up = Some b) /\
-  (forall (pkp : Plc), In_set pkp am.(pubKeyPlcs) -> 
-    exists b, Maps.map_get al.(Lib_PubKeys) pkp = Some b).
+Theorem session_config_subset_trans : forall sc1 sc2 sc3,
+  session_config_subset sc1 sc2 ->
+  session_config_subset sc2 sc3 ->
+  session_config_subset sc1 sc3.
+Proof.
+  unfold session_config_subset; intuition.
+Qed.
+
+Fixpoint session_config_supports_exec (t : Term) (sc : Session_Config) : Prop :=
+  match t with
+  | asp a =>
+      match a with
+      | NULL => True
+      | CPY => True
+      | SIG => 
+          forall l targ targid ev,
+          ((exists res, 
+          sc.(aspCb) (asp_paramsC sig_aspid l targ targid) ev = resultC res) \/ 
+          (exists errStr, sc.(aspCb) (asp_paramsC sig_aspid l targ targid) ev = errC (Runtime errStr)))
+      | HSH =>
+          forall l targ targid ev,
+          ((exists res, 
+          sc.(aspCb) (asp_paramsC hsh_aspid l targ targid) ev = resultC res) \/ 
+          (exists errStr, sc.(aspCb) (asp_paramsC hsh_aspid l targ targid) ev = errC (Runtime errStr)))
+      | ENC p =>
+          (forall l targ targid ev,
+          ((exists res, 
+          sc.(aspCb) (asp_paramsC enc_aspid l targ targid) ev = resultC res) \/ 
+          (exists errStr, sc.(aspCb) (asp_paramsC enc_aspid l targ targid) ev = errC (Runtime errStr)))) /\
+          ((exists res, 
+            map_get (sc.(pubkey_map)) p = Some res))
+      | ASPC _ _ (asp_paramsC aspid _ _ _) =>
+          (forall l targ targid ev,
+          ((exists res, 
+          sc.(aspCb) (asp_paramsC aspid l targ targid) ev = resultC res) \/ 
+          (exists errStr, sc.(aspCb) (asp_paramsC aspid l targ targid) ev = errC (Runtime errStr))))
+      end
+  | att p' t' => 
+      (* We only care that we can dispatch it *)
+      ((exists res, map_get (sc.(plc_map)) p' = Some res))
+  | lseq t1 t2 =>
+      exists sc1 sc2,
+      (session_config_supports_exec t1 sc1) /\
+      (session_config_supports_exec t2 sc2) /\
+      session_config_subset sc1 sc /\
+      session_config_subset sc2 sc
+  | bseq _ t1 t2 =>
+      exists sc1 sc2,
+      (session_config_supports_exec t1 sc1) /\
+      (session_config_supports_exec t2 sc2) /\
+      session_config_subset sc1 sc /\
+      session_config_subset sc2 sc
+  | bpar _ t1 t2 =>
+      exists sc1 sc2,
+      (session_config_supports_exec t1 sc1) /\
+      (session_config_supports_exec t2 sc2) /\
+      session_config_subset sc1 sc /\
+      session_config_subset sc2 sc
+  end.
 
 Ltac unfolds :=
   (* repeat monad_unfold; *)
-  repeat unfold manifest_generator, manifest_compiler, generate_ASP_dispatcher, 
-    generate_Plc_dispatcher, generate_PubKey_dispatcher,
-    lib_supports_manifest, aspid_manifest_update,
+  repeat unfold manifest_generator, generate_ASP_dispatcher, 
+    aspid_manifest_update,
     sig_params, hsh_params, enc_params in *;
   simpl in *; 
   repeat (match goal with
       | x : cvm_st |- _ => destruct x
-      | x : AM_Config |- _ => destruct x
-      | x : AM_Library |- _ => destruct x
+      | x : Session_Config |- _ => destruct x
+      | x : Attestation_Session |- _ => destruct x
       | x : CallBackErrors |- _ => destruct x
   end; simpl in *; eauto);
   intuition.
@@ -47,8 +124,24 @@ Proof.
 Qed.
 
 Global Hint Resolve man_gen_aspid_in : core.
+Require Import Manifest_Generator_Union Cvm_Run AM_Manager.
 
-Theorem filter_resolver : forall {A B} `{EqClass A} (m : MapC A B) a (filt : A -> bool),
+
+      (* 
+      In t' (place_terms t tp p) -> 
+      run_cvm_w_config t 
+      (
+        (exists st', 
+          build_cvm (copland_compile t') st = 
+            (resultC tt, st')) 
+        \/
+        (exists st' errStr,
+          build_cvm (copland_compile t') st = 
+            (errC (dispatch_error (Runtime errStr)), st'))
+      )
+    ). *)
+
+(* Theorem filter_resolver : forall {A B} `{EqClass A} (m : MapC A B) a (filt : A -> bool),
   (exists x, map_get m a = Some x) ->
   filt a = true ->
   exists x, map_get (minify_mapC m filt) a = Some x.
@@ -92,8 +185,8 @@ Proof.
 Qed.
 
 Global Hint Resolve filter_resolver : core.
+*)
 
-Require Import Helpers_CvmSemantics.
 
 Ltac kill_map_none :=
   match goal with
@@ -106,7 +199,7 @@ Ltac kill_map_none :=
     let H''' := fresh "H'" in
     eapply H4 in H1 as H';
     destruct H'; find_rewrite; congruence
-  | H1 : In_set ?x ?l,
+  (* | H1 : In_set ?x ?l,
     H3 : map_get (_ ?l' ?fn) ?x = None,
     H4 : forall _ : _, In_set _ ?l -> _
       |- _ => 
@@ -116,145 +209,30 @@ Ltac kill_map_none :=
     eapply H4 in H1 as H';
     assert (H'' : fn x = true) by ff;
     pose proof (filter_resolver _ _ _ H' H'') as H''';
-    destruct H'''; find_rewrite; congruence
+    destruct H'''; find_rewrite; congruence *)
   end.
 
-Lemma callbacks_work_asps : forall absMan amLib amConf aspBin,
-  lib_supports_manifest amLib absMan ->
-  manifest_compiler absMan amLib aspBin = amConf ->
-  (forall x, In_set x absMan.(asps) -> 
-    forall l p t ev res,
-      aspCb amConf (asp_paramsC x l p t) ev = res ->
-      (exists errStr, res = errC (Runtime errStr)) \/ (exists r, res = resultC r)
-  ).
-Proof.
-  induction absMan; simpl in *; intuition;
-  destruct res; eauto; destruct d; eauto.
-  destruct amConf; simpl in *;
-  destruct amLib; simpl in *.
-  unfold manifest_compiler in H0; repeat find_injection;
-  simpl in *; repeat ff; try congruence;
-  unfold lib_supports_manifest in H; intuition; 
-  simpl in *; intuition; eauto; try congruence;
-  kill_map_none.
-Qed.
-
-Lemma never_change_am_conf : forall t st res st',
+Lemma never_change_sess_conf : forall t st res st',
   build_cvm (copland_compile t) st = (res, st') ->
   st_config st = st_config st'.
 Proof.
   intros;
   destruct st.
-  simpl. 
-  edestruct sc_immut.
+  simpl; eauto. 
+  edestruct sc_immut; eauto.
   unfold execErr.
   rewrite H.
-  simpl. eauto.
+  simpl; eauto.
 Qed.
 
-Definition supports_am (ac1 ac2 : AM_Config) : Prop :=
-  (forall aid l targ targid ev, 
-      (forall res, 
-      ac1.(aspCb) (asp_paramsC aid l targ targid) ev = resultC res ->
-      ac2.(aspCb) (asp_paramsC aid l targ targid) ev = resultC res)) /\
-  (forall p, (forall res, 
-      ac1.(pubKeyCb) p = resultC res ->
-      ac2.(pubKeyCb) p = resultC res)) /\
-  (forall p, (forall res, 
-      ac1.(plcCb) p = resultC res ->
-      ac2.(plcCb) p = resultC res)) /\
-  (forall aid l targ targid ev errStr,
-      ac1.(aspCb) (asp_paramsC aid l targ targid) ev = errC (Runtime errStr) ->
-      ac2.(aspCb) (asp_paramsC aid l targ targid) ev = errC (Runtime errStr)) /\
-  (forall p errStr, 
-      ac1.(pubKeyCb) p = errC (Runtime errStr) ->
-      ac2.(pubKeyCb) p = errC (Runtime errStr)) /\
-  (forall p errStr, 
-      ac1.(plcCb) p = errC (Runtime errStr) ->
-      ac2.(plcCb) p = errC (Runtime errStr)) /\
-  (forall a a',
-      map_get ac1.(ASP_to_APPR_ASP_Map) a = Some a' ->
-      map_get ac2.(ASP_to_APPR_ASP_Map) a = Some a') /\
-  (forall a,
-      map_get ac1.(ASP_to_APPR_ASP_Map) a = None ->
-      map_get ac2.(ASP_to_APPR_ASP_Map) a = None).
+Local Hint Resolve never_change_sess_conf : core.
+Local Hint Resolve session_config_subset_refl : core.
+Local Hint Resolve session_config_subset_trans : core.
 
-Theorem supports_am_refl : forall ac1,
-  supports_am ac1 ac1.
-Proof.
-  unfold supports_am; intuition.
-Qed.
-
-Theorem supports_am_trans : forall ac1 ac2 ac3,
-  supports_am ac1 ac2 ->
-  supports_am ac2 ac3 ->
-  supports_am ac1 ac3.
-Proof.
-  unfold supports_am; intuition.
-Qed.
-
-Local Hint Resolve never_change_am_conf : core.
-Local Hint Resolve supports_am_refl : core.
-Local Hint Resolve supports_am_trans : core.
-
-Fixpoint am_config_support_exec (t : Term) 
-    (p : Plc) (ac : AM_Config) : Prop :=
-  match t with
-  | asp a =>
-      match a with
-      | NULL => True
-      | CPY => True
-      | SIG => 
-          forall l targ targid ev,
-          ((exists res, 
-          ac.(aspCb) (asp_paramsC sig_aspid l targ targid) ev = resultC res) \/ 
-          (exists errStr, ac.(aspCb) (asp_paramsC sig_aspid l targ targid) ev = errC (Runtime errStr)))
-      | HSH =>
-          forall l targ targid ev,
-          ((exists res, 
-          ac.(aspCb) (asp_paramsC hsh_aspid l targ targid) ev = resultC res) \/ 
-          (exists errStr, ac.(aspCb) (asp_paramsC hsh_aspid l targ targid) ev = errC (Runtime errStr)))
-      | ENC p =>
-          (forall l targ targid ev,
-          ((exists res, 
-          ac.(aspCb) (asp_paramsC enc_aspid l targ targid) ev = resultC res) \/ 
-          (exists errStr, ac.(aspCb) (asp_paramsC enc_aspid l targ targid) ev = errC (Runtime errStr)))) /\
-          ((exists res, ac.(pubKeyCb) p = resultC res) \/ 
-          (exists errStr, ac.(pubKeyCb) p = errC (Runtime errStr)))
-      | ASPC _ _ (asp_paramsC aspid _ _ _) =>
-          (forall l targ targid ev,
-          ((exists res, 
-          ac.(aspCb) (asp_paramsC aspid l targ targid) ev = resultC res) \/ 
-          (exists errStr, ac.(aspCb) (asp_paramsC aspid l targ targid) ev = errC (Runtime errStr))))
-      end
-  | att p' t' =>
-      ((exists res, ac.(plcCb) p' = resultC res) \/ 
-      (exists errStr, ac.(plcCb) p' = errC (Runtime errStr)))
-      (* /\ am_config_support_exec t' p' ac *)
-  | lseq t1 t2 =>
-      exists ac1 ac2,
-      (am_config_support_exec t1 p ac1) /\
-      (am_config_support_exec t2 p ac2) /\
-      supports_am ac1 ac /\
-      supports_am ac2 ac
-  | bseq _ t1 t2 =>
-      exists ac1 ac2,
-      (am_config_support_exec t1 p ac1) /\
-      (am_config_support_exec t2 p ac2) /\
-      supports_am ac1 ac /\
-      supports_am ac2 ac
-  | bpar _ t1 t2 =>
-      exists ac1 ac2,
-      (am_config_support_exec t1 p ac1) /\
-      (am_config_support_exec t2 p ac2) /\
-      supports_am ac1 ac /\
-      supports_am ac2 ac
-  end.
-
-Theorem well_formed_am_config_impl_executable : forall t p amConf,
-  am_config_support_exec t p amConf ->
+Theorem well_formed_am_config_impl_executable : forall t sc,
+  session_config_supports_exec t sc ->
   forall st,
-  supports_am amConf (st.(st_config)) ->
+  session_config_subset sc (st.(st_config)) ->
   (exists st', 
     build_cvm (copland_compile t) st = (resultC tt, st')) \/
   (exists st' errStr, 
@@ -274,7 +252,7 @@ Proof.
       (* repeat find_rewrite; *)
       simpl in *; subst; intuition; 
       eauto; try congruence);
-    unfold supports_am, sig_params, enc_params, hsh_params in *; intuition;
+    unfold session_config_subset, sig_params, enc_params, hsh_params in *; intuition;
 
 
     match goal with
@@ -314,36 +292,15 @@ Proof.
       (* repeat find_rewrite; *)
       simpl in *; subst; intuition; 
       eauto; try congruence);
-    unfold supports_am in *; intuition.
-    +
-      destruct H0; 
-      erewrite H2 in *; try congruence; eauto.
-  - subst; simpl in *; try rewrite eqb_refl in *;
-    repeat (
-      unfold remote_session, doRemote, doRemote_session', do_remote, check_cvm_policy in *;
-      try break_match;
-      try monad_unfold;
-      try break_match
-      try find_injection;
-      try find_contradiction;
-      try find_injection;
-      destruct_conjs;
-      (* repeat find_rewrite; *)
-      simpl in *; subst; intuition; 
-      destruct_conjs;
-      eauto; try congruence);
-    unfold supports_am in *; intuition.
-    match goal with
-    | H : forall _ _, (plcCb ?ac1 _ = errC _ -> plcCb ?ac2 _ = errC _) |- _ =>
-      match goal with
-      | H1 : plcCb ac1 _ = errC _ ,
-        H2 : plcCb ac2 _ = errC _ |- _ =>
-          let H' := fresh "H'" in
-          pose proof (H _ _ H1) as H';
-          rewrite H2 in H';
-          try find_injection; eauto
-      end
-    end.
+    unfold session_config_subset in *; intuition.
+    + break_exists;  
+      repeat find_apply_hyp_hyp; repeat find_rewrite; congruence.
+  - break_exists; intuition.
+    eapply IHt1 in H1; intuition; eauto;
+    monad_unfold; break_exists; find_rewrite; eauto.
+    find_eapply_lem_hyp sc_immut_better; find_rewrite.
+    eapply IHt2 in H; intuition; eauto; break_exists;
+    repeat find_rewrite; eauto.
   - subst; simpl in *; try rewrite eqb_refl in *;
     repeat (
       try break_match;
@@ -356,7 +313,7 @@ Proof.
       simpl in *; subst; intuition; 
       eauto; try congruence);
       match goal with
-      | H1 : exists _ _ : AM_Config, _
+      | H1 : exists _ _ : Session_Config, _
         |- _ =>
           let ac1 := fresh "ac" in
           let ac2 := fresh "ac" in
@@ -370,31 +327,37 @@ Proof.
           | H2 : build_cvm (copland_compile t1) ?st = _
             |- _ =>
               let A := fresh "A" in
-              assert (A : supports_am ac1 (st_config st)); [ 
+              assert (A : session_config_subset ac1 (st_config st)); [
                 simpl in *; eauto
                 |
-                destruct (IHt1 p ac1 AS1 st A);
-                intuition; repeat find_rewrite;
+                destruct (IHt1 ac1 AS1 st A); 
+                intuition; repeat find_rewrite; 
+                try break_exists;
                 repeat find_injection;
                 try congruence; eauto
-              ]
-          end;
+              ];
+            eapply sc_immut_better in H2; simpl in *; 
+            repeat find_rewrite; subst; eauto
+          end
+          ;
           match goal with
           | H3 : build_cvm (copland_compile t2) ?st = _
             |- _ =>
               let A := fresh "A" in
-              assert (A : supports_am ac2 (st_config st)); [ 
+              assert (A : session_config_subset ac2 (st_config st)); [ 
                 repeat find_eapply_lem_hyp never_change_am_conf;
                 repeat find_rewrite;
                 simpl in *; eauto
                 |
-                destruct (IHt2 p ac2 AS2 st A);
+                destruct (IHt2 ac2 AS2 st A);
                 intuition; repeat find_rewrite;
                 repeat find_injection;
                 try congruence; eauto
-              ]
+              ];
+            eapply sc_immut_better in H3; simpl in *; 
+            repeat find_rewrite; subst; eauto
           end
-      end. 
+      end.
   - subst; simpl in *; try rewrite eqb_refl in *;
     repeat (
       try break_match;
@@ -406,123 +369,85 @@ Proof.
       (* repeat find_rewrite; *)
       simpl in *; subst; intuition; 
       eauto; try congruence);
-    match goal with
-    | H1 : exists _ _ : AM_Config, _
-      |- _ =>
-        let ac1 := fresh "ac" in
-        let ac2 := fresh "ac" in
-        let AS1 := fresh "AS" in
-        let AS2 := fresh "AS" in
-        let S1 := fresh "S" in
-        let S2 := fresh "S" in
-        destruct H1 as [ac1 [ac2 [AS1 [AS2 [S1 S2]]]]]
-        ;
-        match goal with
-        | H2 : build_cvm (copland_compile t1) ?st = _
-          |- _ =>
-            let A := fresh "A" in
-            assert (A : supports_am ac1 (st_config st)); [ 
-              simpl in *; eauto
-              |
-              destruct (IHt1 p ac1 AS1 st A);
-              intuition; repeat find_rewrite;
-              repeat find_injection;
-              try congruence; eauto
-            ]
-        end;
-        match goal with
-        | H3 : build_cvm (copland_compile t2) ?st = _
-          |- _ =>
-            let A := fresh "A" in
-            assert (A : supports_am ac2 (st_config st)); [ 
-              repeat find_eapply_lem_hyp never_change_am_conf;
-              repeat find_rewrite;
-              simpl in *; eauto
-              |
-              destruct (IHt2 p ac2 AS2 st A);
-              intuition; repeat find_rewrite;
-              repeat find_injection;
-              try congruence; eauto
-            ]
-        end;
-        repeat find_rewrite; eauto
-    end.
-  - subst; simpl in *; try rewrite eqb_refl in *;
-    repeat (
-      try break_match;
-      try monad_unfold;
-      try break_match
-      try find_injection;
-      try find_contradiction;
-      try find_injection;
-      (* repeat find_rewrite; *)
-      simpl in *; subst; intuition; 
-      eauto; try congruence);
-    match goal with
-    | H1 : exists _ _ : AM_Config, _
-      |- _ =>
-        let ac1 := fresh "ac" in
-        let ac2 := fresh "ac" in
-        let AS1 := fresh "AS" in
-        let AS2 := fresh "AS" in
-        let S1 := fresh "S" in
-        let S2 := fresh "S" in
-        destruct H1 as [ac1 [ac2 [AS1 [AS2 [S1 S2]]]]]
-        ;
-        match goal with
-        | H2 : build_cvm (copland_compile t1) ?st = _
-          |- _ =>
-            let A := fresh "A" in
-            assert (A : supports_am ac1 (st_config st)); [ 
-              simpl in *; eauto
-              |
-              destruct (IHt1 p ac1 AS1 st A);
-              intuition; repeat find_rewrite;
-              repeat find_injection;
-              try congruence; eauto
-            ]
-        end;
-        match goal with
-        | H3 : build_cvm (copland_compile t2) ?st = _
-          |- _ =>
-            let A := fresh "A" in
-            assert (A : supports_am ac2 (st_config st)); [ 
-              repeat find_eapply_lem_hyp never_change_am_conf;
-              repeat find_rewrite;
-              simpl in *; eauto
-              |
-              destruct (IHt2 p ac2 AS2 st A);
-              intuition; repeat find_rewrite;
-              repeat find_injection;
-              try congruence; eauto
-            ]
-        end;
-        repeat find_rewrite; eauto
-    end.
-  (* Unshelve. (* Weirdly, we have trivial existentials left *)
-  all: try (eapply default_bs); try (eapply default_UUID). *)
+      match goal with
+      | H1 : exists _ _ : Session_Config, _
+        |- _ =>
+          let ac1 := fresh "ac" in
+          let ac2 := fresh "ac" in
+          let AS1 := fresh "AS" in
+          let AS2 := fresh "AS" in
+          let S1 := fresh "S" in
+          let S2 := fresh "S" in
+          destruct H1 as [ac1 [ac2 [AS1 [AS2 [S1 S2]]]]]
+          ;
+          match goal with
+          | H2 : build_cvm (copland_compile t1) ?st = _
+            |- _ =>
+              let A := fresh "A" in
+              assert (A : session_config_subset ac1 (st_config st)); [
+                simpl in *; eauto
+                |
+                destruct (IHt1 ac1 AS1 st A); 
+                intuition; repeat find_rewrite; 
+                try break_exists;
+                repeat find_injection;
+                try congruence; eauto
+              ];
+            eapply sc_immut_better in H2; simpl in *; 
+            repeat find_rewrite; subst; eauto
+          end
+          ;
+          match goal with
+          | H3 : build_cvm (copland_compile t2) ?st = _
+            |- _ =>
+              let A := fresh "A" in
+              assert (A : session_config_subset ac2 (st_config st)); [ 
+                repeat find_eapply_lem_hyp never_change_am_conf;
+                repeat find_rewrite;
+                simpl in *; eauto
+                |
+                destruct (IHt2 ac2 AS2 st A);
+                intuition; repeat find_rewrite;
+                repeat find_injection;
+                try congruence; eauto
+              ];
+            eapply sc_immut_better in H3; simpl in *; 
+            repeat find_rewrite; subst; eauto
+          end
+      end.
 Qed.
 
-Definition manifest_support_am_config (m : Manifest) (ac : AM_Config) : Prop :=
+Definition manifest_support_session_conf (m : Manifest) (sc : Session_Config)
+    : Prop :=
   (forall a, In_set a (m.(asps)) -> 
     forall l targ targid ev,
-    (exists res, ac.(aspCb) (asp_paramsC a l targ targid) ev = resultC res) \/
-    (exists errStr, ac.(aspCb) (asp_paramsC a l targ targid) ev = errC (Runtime errStr))) /\
-  (forall p, In_set p (m.(uuidPlcs)) ->
-    (exists res, ac.(plcCb) p = resultC res) \/
-    (exists errStr, ac.(plcCb) p = errC (Runtime errStr))) /\
-  (forall p, In_set p (m.(pubKeyPlcs)) ->
-    (exists res, ac.(pubKeyCb) p = resultC res) \/
-    (exists errStr, ac.(pubKeyCb) p = errC (Runtime errStr))).
+    (exists res, sc.(aspCb) (asp_paramsC a l targ targid) ev = resultC res) \/
+    (exists errStr, sc.(aspCb) (asp_paramsC a l targ targid) ev = errC (Runtime errStr))) /\
+  (forall a, In_set a (m.(asps)) -> 
+    exists loc, map_get (m.(ASP_Mapping)) a = Some loc).
+(* 
+Definition att_sess_support_session_conf (ats : Attestation_Session) (sc : Session_Config)
+    : Prop :=
+  (forall p, 
+    exists res, map_get (att_sess.(plc_map)) p = Some res) /\
+  (forall p, 
+    exists res, map_get (sc.(pubkey_map)) p = Some res). *)
 
-Theorem manifest_support_am_config_compiler : forall absMan amLib aspBin,
-  lib_supports_manifest amLib absMan ->
-  manifest_support_am_config absMan (manifest_compiler absMan amLib aspBin).
+(* 
+Theorem manifest_support_session_conf_compiler 
+    : forall absMan aspBin myUUID att_sess,
+  manifest_support_session_conf 
+    absMan 
+    (session_config_compiler (mkAM_Man_Conf absMan aspBin myUUID) att_sess).
 Proof.
-  unfold lib_supports_manifest, manifest_support_am_config, 
-    manifest_compiler, generate_PubKey_dispatcher, generate_Plc_dispatcher in *;
+  unfold manifest_support_session_conf; intuition.
+  unfold manifest_support_session_conf, session_config_compiler in *;
+  intuition; simpl in *; ff; intuition; eauto.
+  ff.
+  ff.
+  simpl in *; ff; intuition.
   simpl in *; repeat ff; intuition;
-  repeat break_match; simpl in *; eauto with *; intuition; eauto;
+  repeat break_match; simpl in *; eauto with *; intuition; eauto.
   try kill_map_none;
   match goal with
   | H:  context[ map_get (minify_mapC ?l ?filt) ?a],
@@ -546,7 +471,34 @@ Proof.
       rewrite H in CO; destruct CO; congruence
     ]
   end.
-Qed.
+Qed. *)
+
+Fixpoint att_sess_supports_term (ats : Attestation_Session) (t : Term) 
+    : Prop :=
+  match t with
+  | asp a =>
+      match a with
+      | ENC p => 
+        exists v, map_get (ats.(PubKey_Mapping)) p = Some v
+      | _ => True
+      end
+  | att p' t' => 
+      exists v, map_get (ats.(Plc_Mapping)) p' = Some v /\
+      att_sess_supports_term ats t'
+  | lseq t1 t2 =>
+      att_sess_supports_term ats t1 /\
+      att_sess_supports_term ats t2
+  | bseq _ t1 t2 =>
+      att_sess_supports_term ats t1 /\
+      att_sess_supports_term ats t2
+  | bpar _ t1 t2 =>
+      att_sess_supports_term ats t1 /\
+      att_sess_supports_term ats t2
+  end.
+
+Definition well_formed_manifest (m : Manifest) : Prop :=
+  (forall a, In_set a (m.(asps)) -> 
+    (exists v, map_get (m.(ASP_Mapping)) a = Some v)).
 
 Fixpoint manifest_support_term (m : Manifest) (t : Term) : Prop :=
   match t with
@@ -559,13 +511,12 @@ Fixpoint manifest_support_term (m : Manifest) (t : Term) : Prop :=
       | HSH =>
           In_set hsh_aspid (m.(asps))
       | ENC p =>
-          In_set enc_aspid (m.(asps)) /\
-          In_set p (m.(pubKeyPlcs))
+          In_set enc_aspid (m.(asps))
       | ASPC _ _ (asp_paramsC aspid _ _ _) =>
           In_set aspid (m.(asps))
       end
-  | att p' t' =>
-      In_set p' (m.(uuidPlcs))
+  | att p' t' => True
+    (* exists m', manifest_support_term m' t' *)
   | lseq t1 t2 =>
       manifest_support_term m t1 /\
       manifest_support_term m t2
@@ -577,24 +528,28 @@ Fixpoint manifest_support_term (m : Manifest) (t : Term) : Prop :=
       manifest_support_term m t2
   end.
 
-Theorem manifest_support_am_config_impl_am_config: forall t p absMan amConf,
-  manifest_support_am_config absMan amConf ->
+Theorem manifest_support_am_config_impl_am_config: forall t absMan ats,
+  well_formed_manifest absMan ->
   manifest_support_term absMan t ->
-  am_config_support_exec t p amConf.
+  att_sess_supports_term ats t ->
+  forall aspBin uuid,
+  session_config_supports_exec 
+    t 
+    (session_config_compiler (mkAM_Man_Conf absMan aspBin uuid) ats).
 Proof.
+  unfold manifest_support_term, well_formed_manifest in *;
   induction t; simpl in *; intuition; eauto;
-  unfold manifest_support_am_config in *; intuition; eauto;
-  repeat (try break_match; simpl in *; intuition; eauto).
-  - pose proof (IHt1 p absMan amConf); 
-    pose proof (IHt2 p absMan amConf); intuition;
-    exists amConf, amConf; eauto.
-  - pose proof (IHt1 p absMan amConf); 
-    pose proof (IHt2 p absMan amConf); intuition;
-    exists amConf, amConf; eauto.
-  - pose proof (IHt1 p absMan amConf); 
-    pose proof (IHt2 p absMan amConf); intuition;
-    exists amConf, amConf; eauto.
+  repeat match goal with
+  | H : forall _ _, ?p _ _ -> _,
+    H' : ?p _ _ |- _ =>
+      eapply H in H'; intuition; eauto
+  end; try (repeat eexists; eauto; fail).
+  - repeat (break_match; repeat find_rewrite; repeat find_injection;
+      simpl in *; intuition; eauto; break_exists; try congruence);
+    find_apply_hyp_hyp; break_exists; congruence.
+  - break_exists; intuition; eauto.
 Qed.
+Require Import ManCompSoundness_Helpers.
 
 Lemma places_decomp: forall t1 t2 p tp,
 In p (places' t2 (places' t1 [])) -> 
@@ -633,277 +588,44 @@ eauto.
 Qed.
 
 Lemma has_manifest_env_places_env_has_manifest' : forall t p tp m e,
-map_get (manifest_generator' tp t e) p = Some m ->
-(exists m', map_get e p = Some m') \/ 
-In p (places tp t).
+  map_get (manifest_generator' tp t e) p = Some m ->
+  (exists m', map_get e p = Some m') \/ 
+  In p (places tp t).
 Proof.
-
-intros.
-generalizeEverythingElse t.
-induction t; intros.
--
-  destruct a; ff.
-  +
-    unfold asp_manifest_generator in *.
-    unfold asp_manifest_update in *.
-    unfold manifest_update_env in *.
-    ff.
-    ++
-
-    destruct (eq_plc_dec tp p); try solve_by_inversion.
-    left.
-    eexists.
-    eapply mapC_get_distinct_keys_from_set.
-    eassumption.
-    eassumption. 
-
-    ++
-    destruct (eq_plc_dec tp p); try solve_by_inversion.
-    left.
-    eexists.
-    eapply mapC_get_distinct_keys_from_set.
-    eassumption.
-    eassumption.
-    +
-    unfold asp_manifest_generator in *.
-    unfold asp_manifest_update in *.
-    unfold manifest_update_env in *.
-    ff.
-    ++
-
-    destruct (eq_plc_dec tp p); try solve_by_inversion.
-    left.
-    eexists.
-    eapply mapC_get_distinct_keys_from_set.
-    eassumption.
-    eassumption. 
-
-    ++
-    destruct (eq_plc_dec tp p); try solve_by_inversion.
-    left.
-    eexists.
-    eapply mapC_get_distinct_keys_from_set.
-    eassumption.
-    eassumption.
-    +
-    unfold asp_manifest_generator in *.
-    unfold asp_manifest_update in *.
-    unfold manifest_update_env in *.
-    ff.
-    ++
-
-    destruct (eq_plc_dec tp p); try solve_by_inversion.
-    left.
-    eexists.
-    eapply mapC_get_distinct_keys_from_set.
-    eassumption.
-    eassumption. 
-
-    ++
-    destruct (eq_plc_dec tp p); try solve_by_inversion.
-    left.
-    eexists.
-    eapply mapC_get_distinct_keys_from_set.
-    eassumption.
-    eassumption.
-    +
-    unfold asp_manifest_generator in *.
-    unfold asp_manifest_update in *.
-    unfold manifest_update_env in *.
-    ff.
-    ++
-
-    destruct (eq_plc_dec tp p); try solve_by_inversion.
-    left.
-    eexists.
-    eapply mapC_get_distinct_keys_from_set.
-    eassumption.
-    eassumption. 
-
-    ++
-    destruct (eq_plc_dec tp p); try solve_by_inversion.
-    left.
-    eexists.
-    eapply mapC_get_distinct_keys_from_set.
-    eassumption.
-    eassumption.
-    +
-    unfold asp_manifest_generator in *.
-    unfold asp_manifest_update in *.
-    unfold manifest_update_env in *.
-    ff.
-    ++
-
-    destruct (eq_plc_dec tp p); try solve_by_inversion.
-    left.
-    eexists.
-    eapply mapC_get_distinct_keys_from_set.
-    eassumption.
-    eassumption. 
-
-    ++
-    destruct (eq_plc_dec tp p); try solve_by_inversion.
-    left.
-    eexists.
-    eapply mapC_get_distinct_keys_from_set.
-    eassumption.
-    eassumption.
-    +
-    unfold asp_manifest_generator in *.
-    unfold asp_manifest_update in *.
-    unfold manifest_update_env in *.
-    ff.
-    ++
-
-    destruct (eq_plc_dec tp p); try solve_by_inversion.
-    left.
-    eexists.
-    eapply mapC_get_distinct_keys_from_set.
-    eassumption.
-    eassumption. 
-
-    ++
-    destruct (eq_plc_dec tp p); try solve_by_inversion.
-    left.
-    eexists.
-    eapply mapC_get_distinct_keys_from_set.
-    eassumption.
-    eassumption.
-  -
-  unfold manifest_generator in H.
-  simpl in H.
-  unfold at_manifest_generator in *.
-  ff.
-  unfold manifest_generator in IHt.
-
-  destruct (eq_plc_dec tp p0); try solve_by_inversion.
-  destruct (eq_plc_dec p p0); try solve_by_inversion.
-
-  apply IHt in H.
-  door.
-  +
-    unfold manifest_update_env in *.
-    ff; try solve_by_inversion.
-    ++
-    unfold knowsof_manifest_update in *.
-    ff.
-    subst.
-    ff.
-    left.
-    eexists.
-    eapply mapC_get_distinct_keys_from_set.
-    apply n. 
-    eassumption.
-    ++
-    left. 
-    eexists.
-    eapply mapC_get_distinct_keys_from_set.
-    apply n. 
-    eassumption.
-  +
-    door; try solve_by_inversion.
+  intros.
+  generalizeEverythingElse t.
+  induction t; intros.
+  - destruct a; ff;
+    unfold asp_manifest_update, manifest_update_env in *;
+    simpl in *;
+    destEq tp p; eauto;
+    try rewrite map_distinct_key_rw in *; eauto.
+  - simpl in *; intuition; eauto.
+    find_apply_hyp_hyp; intuition.
   - (* lseq case *)
-    ff.
-
-    find_apply_hyp_hyp.
-
-    door.
-    +
-      find_apply_hyp_hyp.
-      door.
-      ++
-      left.
-      eauto.
-      ++
-      right.
-      door; eauto.
-      right.
-
-      eapply places'_cumul.
-      eassumption.
-    +
-      door.
-      ++
-      right.
-      eauto.
-      ++
-      right.
-      right.
-      eapply places_app_cumul.
-      eassumption.
-      unfold not in *.
-      intros.
-      solve_by_inversion.
-  -
-  ff.
-
-  find_apply_hyp_hyp.
-
-  door.
-  +
-    find_apply_hyp_hyp.
-    door.
-    ++
-    left.
+    ff; find_apply_hyp_hyp; intuition;
+    break_exists; eauto;
+    try find_apply_hyp_hyp; intuition;
+    pose proof places'_cumul;
+    pose proof places_app_cumul;
     eauto.
-    ++
-    right.
-    door; eauto.
-    right.
-
-    eapply places'_cumul.
-    eassumption.
-  +
-    door.
-    ++
-    right.
+  - ff; find_apply_hyp_hyp; intuition;
+    break_exists; eauto;
+    try find_apply_hyp_hyp; intuition;
+    pose proof places'_cumul;
+    pose proof places_app_cumul;
     eauto.
-    ++
-    right.
-    right.
-    eapply places_app_cumul.
-    eassumption.
-    unfold not in *.
-    intros.
-    solve_by_inversion.
-
-  -
-  ff.
-
-  find_apply_hyp_hyp.
-
-  door.
-  +
-    find_apply_hyp_hyp.
-    door.
-    ++
-    left.
+  - ff; find_apply_hyp_hyp; intuition;
+    break_exists; eauto;
+    try find_apply_hyp_hyp; intuition;
+    pose proof places'_cumul;
+    pose proof places_app_cumul;
     eauto.
-    ++
-    right.
-    door; eauto.
-    right.
-
-    eapply places'_cumul.
-    eassumption.
-  +
-    door.
-    ++
-    right.
-    eauto.
-    ++
-    right.
-    right.
-    eapply places_app_cumul.
-    eassumption.
-    unfold not in *.
-    intros.
-    solve_by_inversion.
 Qed.
 
 Lemma has_manifest_env_places_env_has_manifest : forall t p tp m,
-map_get (manifest_generator t tp) p = Some m ->
-In p (places tp t).
+  map_get (manifest_generator t tp) p = Some m ->
+  In p (places tp t).
 Proof.
   intros.
   unfold manifest_generator in *.
@@ -912,33 +634,37 @@ Proof.
   door; ff. 
 Qed.
 
-Lemma places_env_has_manifest : forall t p tp e,
-In p (places tp t) -> 
-exists m, 
-map_get (manifest_generator' tp t e) p = Some m.
+
+Lemma places_env_has_manifest : forall t p tp,
+  In p (places tp t) -> 
+  exists m, 
+    map_get (manifest_generator t tp) p = Some m.
 Proof.
   intros.
+  unfold manifest_generator.
   generalizeEverythingElse t.
   induction t; intros.
   -
     ff.
     door; try solve_by_inversion.
     subst.
-    destruct a; 
-    unfold asp_manifest_generator;
+    destruct a;
     unfold asp_manifest_update;
     unfold manifest_update_env;
-    ff;
-    eexists;
-    eapply mapC_get_works.
+    ff; rewrite String.eqb_refl in *; try congruence;
+    eauto.
 
   - (* at case *)
+    simpl in *; intuition; subst; eauto.
+    intuition; subst; eauto.
+    eapply IHt.
+    eapply IHt; eauto.
+    simpl in *; intuition; subst; eauto.
+    eauto.
 
     ff.
     door; ff.
     subst.
-    unfold at_manifest_generator.
-    unfold knowsof_manifest_update.
     ff.
     unfold manifest_update_env.
     ff.
@@ -1212,6 +938,8 @@ Proof.
       eauto.
       eauto.
 Qed.
+*)
+
 
 
 
@@ -1280,46 +1008,24 @@ Proof.
   ff.
   eauto.
 Qed.
+*)
 
 Lemma manifest_supports_term_sub : forall m1 m2 t,
-manifest_subset m1 m2 ->
-manifest_support_term m1 t -> 
-manifest_support_term m2 t.
+  manifest_subset m1 m2 ->
+  manifest_support_term m1 t -> 
+  manifest_support_term m2 t.
 Proof.
   intros.
   generalizeEverythingElse t.
-  induction t; intros.
-  - (* asp case *)
-    ff.
-    ff.
-    subst.
-    unfold manifest_subset in *.
-    destruct_conjs.
-    eauto.
-  - (* at case *)
-    ff.
-    unfold manifest_subset in *.
-    destruct_conjs.
-    eauto.
-  - (* lseq case *)
-    ff.
-    destruct_conjs.
-    split; eauto.
-  - (* bseq case *)
-    ff.
-    destruct_conjs.
-    split; eauto.
-  - (* bpar case *)
-    ff.
-    destruct_conjs.
-    split; eauto.
+  induction t; simpl in *; intuition; eauto;
+  repeat ff. 
 Qed.
 
 Lemma env_subset_man_subset : forall e1 e2 p m m',
-Environment_subset e1 e2 -> 
-map_get e1 p = Some m -> 
-map_get e2 p = Some m' -> 
-manifest_subset m m'.
+  Environment_subset e1 e2 -> 
+  map_get e1 p = Some m -> 
+  map_get e2 p = Some m' -> 
+  manifest_subset m m'.
 Proof.
   intros.
   unfold Environment_subset in *.
@@ -1330,28 +1036,6 @@ Proof.
   ff.
 Qed.
 
-Lemma fdsa : forall e e2 p p0 m absMan,
-Environment_subset
-  (map_set e p0 m) 
-  (e2) -> 
-map_get e2 p0 = Some absMan -> 
-In_set p (uuidPlcs m) -> 
-In_set p (uuidPlcs absMan).
-Proof.
-  intros.
-  assert (map_get (map_set e p0 m) p0 = Some m).
-  {
-    eapply mapC_get_works; eauto.
-  }
-  assert (manifest_subset m absMan).
-  {
-    eapply env_subset_man_subset; eauto.
-  }
-
-  unfold manifest_subset in *.
-  destruct_conjs.
-  eauto.
-Qed.
 
 Theorem man_gen_old_always_supports : forall t t' tp p backMan absMan,
   map_get (manifest_generator' tp t backMan) p = Some absMan ->
@@ -1359,11 +1043,173 @@ Theorem man_gen_old_always_supports : forall t t' tp p backMan absMan,
   In t' (place_terms t tp p) ->
   manifest_support_term absMan t'.
 Proof.
-
   induction t; intuition.
+  - admit. 
+  - simpl in *; intuition; subst; eauto. 
+    * rewrite String.eqb_refl in *; simpl in *; intuition; subst; eauto;
+      simpl in *; eauto.
+    * ff; intuition; subst; eauto; simpl in *; eauto. 
+    * ff; intuition; subst; simpl in *; eauto.
+  - 
+ 
+  ff.
+  ff.
+  +
+  door; try solve_by_inversion.
+  subst.
+  ff.
+  assert (tp = p).
+  {
+    eapply eqb_eq_plc; eauto.
+  }
+  subst.
+
+
+
+  split.
+  ++
+
+    find_apply_lem_hyp asdf_easy.
+    destruct_conjs.
+
+    eapply manifest_supports_term_sub.
+    eassumption.
+
+
+    eapply IHt1.
+    eassumption.
+    eauto.
+    apply top_plc_refl.
+
+  ++
+  eapply IHt2.
+  eassumption.
+  eauto.
+  apply top_plc_refl.
+
+
+  + (* tp <> p *)
+    destruct H0.
+    ++
+      subst.
+      rewrite eqb_plc_refl in *.
+      solve_by_inversion.
+    ++
+      assert ((In t' (place_terms t1 tp p)) \/ (In t' (place_terms t2 tp p))).
+      {
+        eapply in_app_or; eauto.
+      }
+      clear H1.
+
+      destruct H2.
+      +++ (* In t' (place_terms t1 tp p) *)
+        assert (In p (places tp t1)).
+        {
+          apply in_plc_term.
+          eapply in_not_nil.
+          eassumption.
+        }
+          find_apply_lem_hyp asdf.
+          ++++
+            destruct_conjs.
+            eapply manifest_supports_term_sub.
+            eassumption.
+            eapply IHt1.
+            eassumption.
+            eauto.
+            eassumption.
+
+          ++++
+            right.
+            unfold places in *.
+            invc H2.
+            +++++
+              rewrite eqb_plc_refl in Heqb.
+              solve_by_inversion.
+            +++++
+              eauto.
+      +++ (* In t' (place_terms t2 tp p) *)
+        simpl.
+
+        assert (In p (places tp t2)).
+      {
+        apply in_plc_term.
+        eapply in_not_nil; eauto.
+      }
+
+        eapply IHt2.
+        ++++
+          eassumption.
+        ++++
+          right.
+          unfold places in H2.
+          eauto.
+          invc H2.
+            +++++
+              rewrite eqb_plc_refl in *.
+              solve_by_inversion.
+            +++++
+              eassumption.
+          ++++
+            eassumption.
+ 
+  
+  simpl in *.
+    destruct (map_get (manifest_generator' tp t1 backMan) .
+    simpl in *; intuition; subst; eauto; ff;
+    try rewrite String.eqb_refl in *; simpl in *; eauto;
+    try door; subst; simpl in *; try (exfalso; eauto; congruence).
+    destruct (manifest_g)
+    simpl in *; intuition; subst; eauto; ff;
+    intuition; eauto;
+    try rewrite String.eqb_refl in *; try congruence;
+    subst; simpl in *; intuition; eauto.
+    * eapply IHt in H; eauto.
+      ff; intuition; subst; eauto.
+      simpl in *; eauto.
+    * eapply IHt in H; eauto.
+      ff; intuition; subst; eauto.
+      simpl in *; eauto. 
+
+
+  induction t; simpl in *; intuition; subst; eauto;
+  try rewrite String.eqb_refl in *;
+  simpl in *; intuition; subst; eauto.
+  - admit. 
+  - simpl; eauto. 
+  - eapply IHt; eauto. 
+    ff; intuition; subst; eauto.
+    simpl in *.
+    eexists; eapply IHt.
+
+
+  induction t; intuition; subst; simpl in *;
+  intuition; subst; eauto;
+  try match goal with
+  | H : context[?p =? ?p] |- _ =>
+    rewrite String.eqb_refl in H
+  end; simpl in *; intuition; subst; eauto;  
+  try unfold manifest_update_env, aspid_manifest_update, 
+    asp_manifest_update in *;
+  try rewrite mapC_get_works in *; repeat find_injection;
+  simpl in *; intuition; eauto; repeat (ff; fail).
+  - eapply IHt in H; eauto. 
+  repeat (try break_match; 
+    try unfold manifest_update_env, aspid_manifest_update in *;
+    subst; simpl in *; intuition;
+    subst; repeat find_rewrite; repeat find_injection;
+    try rewrite mapC_get_works in *;
+    eauto using in_set_add, manadd_In_add;
+    intuition; eauto; try congruence);
+  try eapply manadd_In_add.
+    pose proof manadd_In_add; eauto
+    eapply manadd_In_add.
+    pose proof in_set_add.
+    Search manset_add.
+  eauto using in_set_add.
   - repeat (try break_match; 
-      unfold asp_manifest_generator, manifest_update_env, knowsof_manifest_update,
-        aspid_manifest_update, update_manifest_policy_targ, pubkey_manifest_update in *;
+      unfold manifest_update_env, 
+        aspid_manifest_update in *;
       subst; simpl in *; intuition; eauto; try congruence;
       repeat find_rewrite;
       repeat find_injection;
@@ -1371,8 +1217,17 @@ Proof.
     try (rewrite mapC_get_works in *; simpl in *; repeat find_injection; simpl in *; intuition; eauto);
     try (eapply manadd_In_add).
 
-
   - (* at case *)
+    simpl in *; intuition; subst; eauto;
+    eapply IHt in H; intuition; subst; eauto.
+    * ff; intuition; subst; eauto.
+      ** admit.
+      **  destEq p0 p0; eauto.
+      rewrite eqb_refl in *.
+    eapply IHt in H; intuition; subst; eauto;
+    break_if; intuition; simpl in *; intuition;
+    subst.
+    repeat ff; intuition; subst; eauto.
   ff.
 
   ff.
@@ -1741,20 +1596,42 @@ Proof.
         ++++
           eassumption.
 Qed.
+*)
 
-Theorem manifest_generator_compiler_soundness_distributed : forall t tp p absMan amLib amConf aspBin,
+Lemma att_sess_supports_place_terms : forall ats t tp p t',
+  att_sess_supports_term ats t ->
+  In t' (place_terms t tp p) ->
+  att_sess_supports_term ats t'.
+Proof.
+  induction t; simpl in *; intuition; eauto;
+  repeat (ff; subst; simpl in *; repeat find_rewrite;
+    repeat find_injection; intuition; eauto).
+  - break_exists; intuition.
+    eapply IHt in H2; eauto.
+  - find_eapply_lem_hyp in_app_iff; intuition; eauto.
+  - find_eapply_lem_hyp in_app_iff; intuition; eauto.
+  - find_eapply_lem_hyp in_app_iff; intuition; eauto.
+Qed.
+
+Lemma man_gen_yields_wf_manifests : forall t tp p absMan,
+  (* well_formed_manifest backMan -> *)
+  map_get (manifest_generator' tp t []) p = Some absMan ->
+  well_formed_manifest absMan.
+Proof.
+  induction t; simpl in *; intuition; eauto;
+  repeat ff; intuition; simpl in *.
+  - unfold well_formed_manifest; intuition. 
+    unfold asp_manifest_update; simpl in *; ff; intuition;
+    subst; eauto.
+
+Theorem manifest_generator_compiler_soundness_distributed : forall t tp p absMan uuid aspBin sc att_sess,
   map_get (manifest_generator t tp) p = Some absMan ->
-  lib_supports_manifest amLib absMan ->
-  manifest_compiler absMan amLib aspBin = amConf ->
+  well_formed_manifest absMan ->
+  manifest_support_session_conf absMan sc ->
+  att_sess_supports_term att_sess t ->
+  session_config_compiler (mkAM_Man_Conf absMan aspBin uuid) att_sess = sc ->
   forall st,
-
-  (* st.(st_config) = amConf -> *)
-
-  
-    (* Note, this should be trivial typically as amConf = st.(st_config) and refl works *)
-    supports_am amConf (st.(st_config)) ->  
-
-
+    session_config_subset sc (st.(st_config)) ->  
     (  forall t', 
          In t' (place_terms t tp p) -> 
         (exists st', 
@@ -1766,13 +1643,16 @@ Theorem manifest_generator_compiler_soundness_distributed : forall t tp p absMan
     ).
 Proof.
   intros.
-  assert (supports_am amConf (st.(st_config))) by ff.
   assert (In p (places tp t)) by 
-            (eapply has_manifest_env_places_env_has_manifest; eauto).
-  eapply well_formed_am_config_impl_executable.
+            (eapply has_manifest_env_places_env_has_manifest; eauto);
+  subst.
+  eapply well_formed_am_config_impl_executable; eauto.
   - unfold manifest_generator, e_empty in *; simpl in *.
-    eapply manifest_support_am_config_impl_am_config.
-    * eapply manifest_support_am_config_compiler; eauto.
+    eapply manifest_support_am_config_impl_am_config; eauto.
+    * 
+    * eapply att_sess_supports_place_terms; eauto.
+      Search (manifest_support_term _ _).
+      eapply manifest_support_am_config_compiler; eauto.
     * (* NOTE: This is the important one, substitute proof of any manifest here *)
       eapply man_gen_old_always_supports.
       eassumption.
@@ -1798,23 +1678,6 @@ Require Import Manifest_Generator_Union.
 
 Close Scope cop_ent_scope.
 
-Lemma manifest_subset_union_l : forall m1 m2,
-  manifest_subset m1 (Manifest_Union.manifest_union_asps m1 m2).
-Proof.
-  induction m1; destruct m2; simpl in *; intuition; eauto;
-  unfold manifest_subset; simpl in *; intuition; eauto;
-  try eapply union_inclusion_l; eauto.
-Qed.
-Global Hint Resolve manifest_subset_union_l : core.
-
-Lemma manifest_subset_union_r : forall m1 m2,
-  manifest_subset m2 (Manifest_Union.manifest_union_asps m1 m2).
-Proof.
-  induction m1; destruct m2; simpl in *; intuition; eauto;
-  unfold manifest_subset; simpl in *; intuition; eauto;
-  try eapply union_inclusion_r; eauto.
-Qed.
-Global Hint Resolve manifest_subset_union_r : core.
 (* Global Hint Resolve manifest_subset_union_l : core. *)
 
 Lemma manifest_env_union_works : forall env env' p m,
@@ -2593,3 +2456,40 @@ Proof.
   eassumption.
 Qed.
 
+Theorem manifest_generator_compiler_soundness_distributed_multiterm 
+    : forall t ts ls tp p comp_map absMan env,
+  end_to_end_mangen comp_map ls ts = resultC env ->
+  map_get env p = Some absMan -> 
+  In (t,tp) ts ->
+  (* lib_supports_manifest amLib absMan -> *)
+  (*
+    (* Note, this should be trivial typically as amConf = st.(st_config) and refl works *)
+    supports_am amConf (st.(st_config)) ->  
+    *)
+  (forall t' att_sess aspBin uuid conf ev,
+    In t' (place_terms t tp p) -> 
+    conf = (mkAM_Man_Conf absMan aspBin uuid) ->
+    (exists st',
+      (run_cvm_w_config t' ev (session_config_compiler conf att_sess)) = 
+      (resultC st')) 
+    \/
+    (exists errStr,
+      (run_cvm_w_config t' ev (session_config_compiler conf att_sess)) = 
+      (errC (dispatch_error (Runtime errStr)))
+    )
+  ).
+Proof.
+  induction t; subst; simpl in *; intuition; subst; eauto;
+  simpl in *; intuition; eauto.
+  - destruct (tp =? p); simpl in *; intuition; subst;
+    simpl in *;
+    unfold run_cvm_w_config, run_cvm, run_core_cvm;
+    destruct a; simpl in *; eauto;
+    repeat (break_match; subst; repeat find_rewrite; repeat find_injection;
+      simpl in *; intuition; eauto; try monad_unfold; try congruence).
+    unfold generate_ASP_dispatcher, generate_ASP_dispatcher' in *; simpl in *; intuition.
+    * unfold generate_ASP_dispatcher, generate_ASP_dispatcher' in *; simpl in *; intuition.  
+      ff; simpl in *.
+      build_cvm; simpl in *.
+
+  subst.
